Refactor as per PR comments
Second of two steps, in src/SDK/MessageHeader:

Rename Format.dfy to MessageHeader.dfy.

Move/rename modules:
* MessageHeader.Format -> MessageHeader
* MessageHeader.Deserialize -> Deserialize
* MessageHeader.Serialize -> Serialize

Move InsertNewEntry method from MessageHeader into Deserialize.

Move serialization specification functions into MessageHeader module.
Change name of SerializeXYZ functions to XYZToSeq.
Remove "Impl" from the names of Serialize methods.

src/SDK/MessageHeader/MessageHeader.dfy
@@ -3,7 +3,7 @@ include "../../StandardLibrary/StandardLibrary.dfy"
 include "../Materials.dfy"
 include "../../Util/UTF8.dfy"
 
-module MessageHeader.Format {
+module MessageHeader {
   import AlgorithmSuite
   import opened StandardLibrary
   import opened UInt = StandardLibrary.UInt
@@ -13,6 +13,7 @@ module MessageHeader.Format {
   /*
    * Definition of the message header, i.e., the header body and the header authentication
    */
+
   datatype Header = Header(body: HeaderBody, auth: HeaderAuthentication)
   {
     predicate Valid() {
@@ -22,10 +23,10 @@ module MessageHeader.Format {
     }
   }
 
-
   /*
    * Header body type definition
    */
+
   const VERSION_1: uint8     := 0x01
   type Version               = x | x == VERSION_1 witness VERSION_1
 
@@ -88,11 +89,15 @@ module MessageHeader.Format {
     }
   }
 
-
   /*
    * Header authentication type definition
    */
+
   datatype HeaderAuthentication = HeaderAuthentication(iv: seq<uint8>, authenticationTag: seq<uint8>)
+
+  /*
+   * Validity predicates -- predicates that say when the data structures above are in a good state.
+   */
 
   predicate ValidKVPair(kvPair: (seq<uint8>, seq<uint8>)) {
     && |kvPair.0| < UINT16_LIMIT
@@ -213,32 +218,126 @@ module MessageHeader.Format {
     SortedKVPairsUpTo(a, |a|)
   }
 
-  method InsertNewEntry(kvPairs: seq<(seq<uint8>, seq<uint8>)>, key: seq<uint8>, value: seq<uint8>)
-      returns (res: Option<seq<(seq<uint8>, seq<uint8>)>>, ghost insertionPoint: nat)
-    requires SortedKVPairs(kvPairs)
-    ensures match res
-    case None =>
-      exists i :: 0 <= i < |kvPairs| && kvPairs[i].0 == key  // key already exists
-    case Some(kvPairs') =>
-      && insertionPoint <= |kvPairs|
-      && kvPairs' == kvPairs[..insertionPoint] + [(key, value)] + kvPairs[insertionPoint..]
-      && SortedKVPairs(kvPairs')
+  /*
+   * Specifications of serialized format
+   */
+
+  function {:opaque} HeaderBodyToSeq(hb: HeaderBody): seq<uint8>
+    requires hb.Valid()
   {
+    [hb.version as uint8] +
+    [hb.typ as uint8] +
+    UInt16ToSeq(hb.algorithmSuiteID as uint16) +
+    hb.messageID +
+    AADToSeq(hb.aad) +
+    EDKsToSeq(hb.encryptedDataKeys) +
+    [ContentTypeToUInt8(hb.contentType)] +
+    hb.reserved +
+    [hb.ivLength] +
+    UInt32ToSeq(hb.frameLength)
+  }
+
+  function AADToSeq(kvPairs: Materials.EncryptionContext): seq<uint8>
+    requires ValidAAD(kvPairs)
+  {
+    reveal ValidAAD();
+    UInt16ToSeq(AADLength(kvPairs) as uint16) +
     var n := |kvPairs|;
-    while 0 < n && LexicographicLessOrEqual(key, kvPairs[n - 1].0, UInt8Less)
-      invariant 0 <= n <= |kvPairs|
-      invariant forall i :: n <= i < |kvPairs| ==> LexicographicLessOrEqual(key, kvPairs[i].0, UInt8Less)
-    {
-      n := n - 1;
-    }
-    if 0 < n && kvPairs[n - 1].0 == key {
-      return None, n;
-    } else {
-      var kvPairs' := kvPairs[..n] + [(key, value)] + kvPairs[n..];
-      if 0 < n {
-        LexPreservesTrichotomy(kvPairs'[n - 1].0, kvPairs'[n].0, UInt8Less);
+    if n == 0 then [] else
+      UInt16ToSeq(n as uint16) +
+      KVPairsToSeq(kvPairs, 0, n)
+  }
+
+  function KVPairsToSeq(kvPairs: Materials.EncryptionContext, lo: nat, hi: nat): seq<uint8>
+    requires forall i :: 0 <= i < |kvPairs| ==> ValidKVPair(kvPairs[i])
+    requires lo <= hi <= |kvPairs|
+  {
+    if lo == hi then [] else KVPairsToSeq(kvPairs, lo, hi - 1) + KVPairToSeq(kvPairs[hi - 1])
+  }
+
+  function KVPairToSeq(kvPair: (seq<uint8>, seq<uint8>)): seq<uint8>
+    requires ValidKVPair(kvPair)
+  {
+    UInt16ToSeq(|kvPair.0| as uint16) + kvPair.0 +
+    UInt16ToSeq(|kvPair.1| as uint16) + kvPair.1
+  }
+
+  function EDKsToSeq(encryptedDataKeys: EncryptedDataKeys): seq<uint8>
+    requires encryptedDataKeys.Valid()
+  {
+    var n := |encryptedDataKeys.entries|;
+    UInt16ToSeq(n as uint16) +
+    EDKEntriesToSeq(encryptedDataKeys.entries, 0, n)
+  }
+
+  function EDKEntriesToSeq(entries: seq<Materials.EncryptedDataKey>, lo: nat, hi: nat): seq<uint8>
+    requires forall i :: 0 <= i < |entries| ==> entries[i].Valid()
+    requires lo <= hi <= |entries|
+  {
+    if lo == hi then [] else EDKEntriesToSeq(entries, lo, hi - 1) + EDKEntryToSeq(entries[hi - 1])
+  }
+
+  function EDKEntryToSeq(edk: Materials.EncryptedDataKey): seq<uint8>
+    requires edk.Valid()
+  {
+    UInt16ToSeq(|edk.providerID| as uint16)   + StringToByteSeq(edk.providerID) +
+    UInt16ToSeq(|edk.providerInfo| as uint16) + edk.providerInfo +
+    UInt16ToSeq(|edk.ciphertext| as uint16)   + edk.ciphertext
+  }
+
+  /* Function AADLength is defined without referring to SerializeAAD (because then
+   * these two would be mutually recursive with ValidAAD). The following lemma proves
+   * that the two definitions correspond.
+   */
+
+  lemma ADDLengthCorrect(kvPairs: Materials.EncryptionContext)
+    requires ValidAAD(kvPairs)
+    ensures |AADToSeq(kvPairs)| == 2 + AADLength(kvPairs)
+  {
+    reveal ValidAAD();
+    KVPairsLengthCorrect(kvPairs, 0, |kvPairs|);
+    /**** Here's a more detailed proof:
+    var n := |kvPairs|;
+    if n != 0 {
+      var s := KVPairsToSeq(kvPairs, 0, n);
+      calc {
+        |AADToSeq(kvPairs)|;
+      ==  // def. AADToSeq
+        |UInt16ToSeq(AADLength(kvPairs) as uint16) + UInt16ToSeq(n as uint16) + s|;
+      ==  // UInt16ToSeq yields length-2 sequence
+        2 + 2 + |s|;
+      ==  { KVPairsLengthCorrect(kvPairs, 0, n); }
+        2 + 2 + KVPairsLength(kvPairs, 0, n);
       }
-      return Some(kvPairs'), n;
     }
+    ****/
+  }
+
+  lemma KVPairsLengthCorrect(kvPairs: Materials.EncryptionContext, lo: nat, hi: nat)
+    requires forall i :: 0 <= i < |kvPairs| ==> ValidKVPair(kvPairs[i])
+    requires lo <= hi <= |kvPairs|
+    ensures |KVPairsToSeq(kvPairs, lo, hi)| == KVPairsLength(kvPairs, lo, hi)
+  {
+    /**** Here's a more detailed proof:
+    if lo < hi {
+      var kvPair := kvPairs[hi - 1];
+      calc {
+        |KVPairsToSeq(kvPairs, lo, hi)|;
+      ==  // def. KVPairsToSeq
+        |KVPairsToSeq(kvPairs, lo, hi - 1) + KVPairToSeq(kvPair)|;
+      ==
+        |KVPairsToSeq(kvPairs, lo, hi - 1)| + |KVPairToSeq(kvPair)|;
+      ==  { KVPairsLengthCorrect(kvPairs, lo, hi - 1); }
+        KVPairsLength(kvPairs, lo, hi - 1) + |KVPairToSeq(kvPair)|;
+      ==  // def. KVPairToSeq
+        KVPairsLength(kvPairs, lo, hi - 1) +
+        |UInt16ToSeq(|kvPair.0| as uint16) + kvPair.0 + UInt16ToSeq(|kvPair.1| as uint16) + kvPair.1|;
+      ==
+        KVPairsLength(kvPairs, lo, hi - 1) + 2 + |kvPair.0| + 2 + |kvPair.1|;
+      ==  // def. KVPairsLength
+        KVPairsLength(kvPairs, lo, hi);
+      }
+    }
+    ****/
   }
 }
